theories/iris/language/lenient_wp.v
@@ -59,38 +59,6 @@ Section lenient_wp.
 
   End wp_params.
 
-  Lemma lenient_wp_seq s E (Φ Ψ: logpred) es1 es2 :
-    lenient_wp NotStuck E es1 Ψ ∗
-    (* trap case: old frame and trap conditions imply the new ones *)
-    (∀ f, lp_trap Ψ ∗ lp_fr Ψ f -∗ lp_trap Φ ∗ lp_fr Φ f) ∗
-    (* non-trap case: old frame and non-trap conditions imply the new wp *)
-    (∀ w f, lp_notrap Ψ w ∗ ↪[frame] f ∗ lp_fr Ψ f -∗ lenient_wp s E (of_val w ++ es2) Φ)
-    ⊢ lenient_wp s E (es1 ++ es2) Φ.
-  Proof.
-    iIntros "(Hes1 & Htrapimpl & Hes2)".
-    iApply (wp_seq_can_trap s E _ (lp_notrap Ψ) _ _ Ψ.(lp_fr) (↪[BAIL] ∗ Ψ.(lp_trap))).
-    iSplitR; [done |].
-    unfold lenient_wp.
-    iSplitL "Htrapimpl".
-    {
-      iIntros (f0) "[Hf0 [[Hbail Htrap] Hfr]]".
-      iFrame.
-      iApply "Htrapimpl".
-      iFrame.
-    }
-    iSplitR "Hes2".
-    - iApply (wp_wand with "[Hes1]").
-      + iApply "Hes1".
-      + iIntros (v). destruct v; unfold denote_logpred; cbn; iIntros "[Hlog Hfr]";
-          try iFrame.
-        iLeft.
-        by iFrame.
-    - iIntros (w f) "(Hnotrap & Hfr & Hfrcond)".
-      iApply "Hes2".
-      iFrame.
-  Qed.
-
-
   Definition sigT_apply {A} {P: A -> Type} (f: forall a, P a -> P a) (x: {a: A & P a}) : {a: A & P a} :=
     existT (projT1 x) (f _ (projT2 x)).
 
