theories/iris/rules/lwp_pure.v
@@ -8,6 +8,25 @@ Section lwp_pure.
   Context `{!wasmG Σ}.
   Open Scope bi_scope.
   
+  Lemma lwp_unop s E Φ op t v v' (f: datatypes.frame) :
+    app_unop op v = v' ->
+    ↪[frame] f ∗
+    ↪[RUN] ∗
+    ▷ Φ.(lp_val) [v'] ∗
+    Φ.(lp_fr) f
+    ⊢ lenient_wp s E [AI_basic (BI_const v); AI_basic (BI_unop t op)] (lp_run Φ).
+  Proof.
+    iIntros (Happ) "(Hf & Hrun & Hval & Hfr)".
+    iApply (wp_wand with "[Hf Hrun Hval]").
+    - iApply (wp_unop with "[$] [$]").
+      eauto.
+      by instantiate (1:= lp_noframe Φ).
+    - iIntros (w) "[[Hnofr Hrun] Hf]".
+      unfold lp_run.
+      rewrite -lp_with_sep.
+      iFrame.
+  Qed.
+
   Lemma lwp_binop s E Φ op t v1 v2 v (f: datatypes.frame) :
     app_binop op v1 v2 = Some v →
     ↪[frame] f ∗
@@ -25,6 +44,23 @@ Section lwp_pure.
       unfold lp_run.
       rewrite -lp_with_sep.
       iFrame.
+  Qed.
+  
+  Lemma lwp_binop_failure s E Φ op t v1 v2 (f: datatypes.frame) :
+    app_binop op v1 v2 = None →
+    ↪[frame] f ∗
+    ↪[RUN] ∗
+    ▷ Φ.(lp_trap) ∗
+    Φ.(lp_fr) f
+    ⊢ lenient_wp s E [AI_basic (BI_const v1); AI_basic (BI_const v2); AI_basic (BI_binop t op)] Φ.
+    iIntros (Happ) "(Hf & Hrun & Htrap & Hfr)".
+    iApply (wp_wand with "[Hf Hrun Htrap]").
+    - iApply (wp_binop_failure with "[Htrap] [$] [$]").
+      eauto.
+      by instantiate (1:= lp_nobail Φ).
+    - iIntros (w) "[[Hbail Hrun] Hf]".
+      destruct w; cbn; try iDestruct "Hbail" as "[]".
+      by iFrame.
   Qed.
 
   Lemma lwp_relop s E Φ op t v1 v2 b (f: datatypes.frame) :
@@ -45,8 +81,56 @@ Section lwp_pure.
       rewrite -lp_with_sep.
       iFrame.
   Qed.
+  
+  Lemma lwp_testop_i32 s E Φ v b op (f: datatypes.frame) :
+    app_testop_i (e:=i32t) op v = b ->
+    ↪[frame] f ∗
+    ↪[RUN] ∗
+    ▷ Φ.(lp_val) [VAL_int32 (wasm_bool b)] ∗
+    Φ.(lp_fr) f
+    ⊢ lenient_wp s E [AI_basic (BI_const (VAL_int32 v)); AI_basic (BI_testop T_i32 op)] (lp_run Φ).
+  Proof.
+  Admitted.
+  
+  Lemma lwp_testop_i64 s E Φ v b op (f: datatypes.frame) :
+    app_testop_i (e:=i64t) op v = b ->
+    ↪[frame] f ∗
+    ↪[RUN] ∗
+    ▷ Φ.(lp_val) [VAL_int32 (wasm_bool b)] ∗
+    Φ.(lp_fr) f
+    ⊢ lenient_wp s E [AI_basic (BI_const (VAL_int64 v)); AI_basic (BI_testop T_i64 op)] (lp_run Φ).
+  Proof.
+  Admitted.
 
-  Lemma lenient_wp_nop s E Φ :
+  Lemma lwp_cvtop_convert s E Φ v v' t1 t2 sx (f: datatypes.frame) :
+    cvt t2 sx v = Some v' ->
+    types_agree t1 v ->
+    ↪[frame] f ∗
+    ↪[RUN] ∗
+    ▷ Φ.(lp_val) [v']
+    ⊢ lenient_wp s E [AI_basic (BI_const v); AI_basic (BI_cvtop t2 CVO_convert t1 sx)] (lp_run Φ).
+  Proof.
+  Admitted.
+
+  Lemma lwp_cvtop_reinterpret s E Φ v v' t1 t2 (f: datatypes.frame) :
+    wasm_deserialise (bits v) t2 = v' ->
+    types_agree t1 v ->
+    ↪[frame] f ∗
+    ↪[RUN] ∗
+    ▷ Φ.(lp_val) [v']
+    ⊢ lenient_wp s E [AI_basic (BI_const v); AI_basic (BI_cvtop t2 CVO_reinterpret t1 None)] (lp_run Φ).
+  Proof.
+  Admitted.
+
+  Lemma lwp_unreachable  s E Φ (f: datatypes.frame) :
+    ↪[frame] f ∗
+    ↪[RUN] ∗
+    ▷ Φ.(lp_trap)
+    ⊢ lenient_wp s E [AI_basic BI_unreachable] Φ.
+  Proof.
+  Admitted.
+
+  Lemma lwp_nop s E Φ :
     ↪[RUN] ∗
     denote_logpred Φ (immV [])
     ⊢ lenient_wp s E [AI_basic BI_nop] (lp_run Φ).
@@ -60,5 +144,37 @@ Section lwp_pure.
     iEval (rewrite -lp_with_sep).
     iFrame.
   Qed.
+
+  Lemma lwp_drop s E Φ v (f: datatypes.frame) :
+    ↪[frame] f ∗
+    ↪[RUN] ∗
+    ▷ Φ.(lp_val) []
+    ⊢ lenient_wp s E [AI_basic (BI_const v); AI_basic BI_drop] (lp_run Φ).
+  Proof.
+  Admitted.
+  
+  Lemma lwp_select_false s E Φ n v1 v2 (f: datatypes.frame) :
+    n = Wasm_int.int_zero i32m ->
+    ↪[frame] f ∗
+    ↪[RUN] ∗
+    ▷ Φ.(lp_val) [v2]
+    ⊢ lenient_wp s E 
+        [AI_basic (BI_const v1); AI_basic (BI_const v2);
+         AI_basic (BI_const (VAL_int32 n)); AI_basic (BI_select)]
+        (lp_run Φ).
+  Proof.
+  Admitted.
+  
+  Lemma lwp_select_true s E Φ n v1 v2 (f: datatypes.frame) :
+    n = Wasm_int.int_zero i32m ->
+    ↪[frame] f ∗
+    ↪[RUN] ∗
+    ▷ Φ.(lp_val) [v1]
+    ⊢ lenient_wp s E 
+        [AI_basic (BI_const v1); AI_basic (BI_const v2);
+         AI_basic (BI_const (VAL_int32 n)); AI_basic (BI_select)]
+        (lp_run Φ).
+  Proof.
+  Admitted.
 
 End lwp_pure.
